Date: 2025-11-05
Tags: 

3/4/4
a)
$$\frac{1}{4\cdot5} + \frac{1}{5 \cdot 6} + \dots + \frac{1}{(n+3)(n+4)} = \frac{n}{4(n+4)}$$
Bizonyítás :
1. $n=1$  $\frac{1}{4\cdot 5} = \frac{1}{4(1+4)}$
2. Tfh. k-ra igaz: 
	$$\frac{1}{4\cdot 5} + \frac{1}{5 \cdot 6} + \dots + \frac{1}{(k+3)(k+4)} = \frac{k}{4\cdot (k+4)}$$
	Megmutatjuk, hogy:
	$$\frac{1}{4\cdot 5} + \frac{1}{5 \cdot 6} + \dots + \frac{1}{(k+3)(k+4)} + \frac{1}{(k+4)(k+5)} = \frac{k+1}{4\cdot (k+4+1)}$$
$$\frac{k}{4\cdot(k+4)} + \frac{1}{(k+4)(k+5)} = \frac{k+1}{4\cdot (k+5)}$$

$$k(k+5)+4=(k+1)(k+4)$$
b)

$$2\cdot 2^1 +3\cdot 2^2 + 4\cdot 2^3 + 5\cdot 2^4$ + \dots + n\cdot 2^{n-1} = (n-1)2^{n}$$
Biz.: 
1. $n=2$  $2\cdot 2^1 = (2-1)2^2$
2. Tfh.: n=k igaz $2\cdot 2^1 + 3\cdot 2^2 + \dots +k\cdot 2^{k-1} = (k-1)2^{k}$
	Lássuk be n= k+1-re:
	$$2\cdot 2^1 + 3\cdot 2^2 + \dots +k\cdot 2^{k-1} + (k+1)\cdot 2^k = k\cdot 2^{k+1}$$$$(k-1)\cdot 2^{k} + (k+1)\cdot 2^k = k\cdot 2^{k+1} $$
