
$f_{0} = 0$
$f_{1} = 3$
$f_{2} = 8$
$f_{3} = 21$

$$f_{n} = 3\cdot f_{n-1} - f_{n-2}$$
$x^{2} = 3\cdot x - 1$

$$x_{1,2} = \frac{3 \pm \sqrt{ 5 }}{2}$$

$3=A \cdot \frac{3 - \sqrt{ 5 }}{2} + B \cdot \frac{3 + \sqrt{ 5 }}{2}$

$8=A \cdot (\frac{3 - \sqrt{ 5 }}{2})^2 + B \cdot (\frac{3 + \sqrt{ 5 }}{2})^2$

$A = \frac {5-3 \sqrt{ 5 }}{10}$
$B = \frac {5+3 \sqrt{ 5 }}{10}$

$$f_{n} = \frac {5-3 \sqrt{ 5 }}{10} \cdot (\frac{3 - \sqrt{ 5 }}{2})^{n} + \frac {5+3 \sqrt{ 5 }}{10} \cdot (\frac{3 + \sqrt{ 5 }}{2})^{n}$$

